\begin{align}
  p_{bag(pos)} & = \pi_{pos}^+ p^+(x|\theta_b^+) + (1-\pi_{pos}^+) p^-(x|\theta_b^-) \\
  p_{bag(neg)} & = \pi_{neg}^+ p^+(x|\theta_b^+) + (1-\pi_{neg}^+) p^-(x|\theta_b^-)
\end{align}

\begin{align}
  B \rightarrow \infty : 
  \sum_{b = 1} ^B p^+(x|\theta_b^+) =  \sum_{b' = 1} ^{B'} p^+(x|\theta_{b'}^+)
\end{align}

% Not true
%\begin{align}
%  \mathcal{X}_{neg}: p_{pos} (x) < p_{neg} (x) = \sum_{b = 1} ^{B} p^-(x|\theta_{b}^-)
% \end{align}

\begin{align}
  \mathcal{X}_{neg}: p_{pos} (x) < p_{neg} (x) 
\end{align}
 
\begin{align}
  \mathcal{X}_{neg}: E(p_{bag(pos)}) < E(p_{bag(neg)})
\end{align}

\begin{align*}
  \int_{\mathcal{X}_{neg}} \frac{p_{pos}(x)}{p_{neg}(x)} p_{bag(pos)}(x) \log \frac{p_{bag(pos)}(x)}{p_{neg}(x)} dx <
   \int_{\mathcal{X}_{neg}} \frac{p_{pos}(x)}{p_{neg}(x)} p_{bag(neg)}(x) \log \frac{p_{bag(neg)}(x)}{p_{neg}(x)} dx
\end{align*}
 